Work on trace eq arm8 vs bir

src/tools/parallelcomposition/instantiations/arm8_vs_bir_comp_attackerScript.sml
@@ -19,12 +19,14 @@ open bir_program_valid_stateTheory;
 open HolBACoreSimps;
 open bir_backlifterTheory;
 open bir_program_multistep_propsTheory;
+open arithmeticTheory;
+open bir_auxiliaryTheory;
 (* HOL_Interactive.toggle_quietdec(); *)
 
 val _ = new_theory "arm8_vs_bir_comp_attacker";
 
 val arm8_rel_def = Define `
-                          arm8_rel ms mev ms' = ((NextStateARM8 ms = SOME ms') ∧ (mev = ((1):num)))`;
+                          arm8_rel ms mev ms' = (FUNPOW_OPT arm8_bmr.bmr_step_fun mev ms = SOME ms')`;
 
 Inductive arm8_mrel:
 [~nil:]
@@ -52,20 +54,21 @@ Define `arm8_mrel ms meve ms' =
                           `;*)
                           
 val bir_rel_def = Define `
-    bir_rel birprog bs bev bs' = ((bs' = bir_exec_step_state birprog bs) ∧ (bev = ((1):num)))
+    bir_rel p bs bev bs' = (∀n' lo c_st. (bir_exec_to_addr_label_n p bs n' =
+        BER_Ended lo c_st bev bs'))
                                  `;
-
+(*
 val bir_mrel_def =
 Define ` (bir_mrel birprog bs ([]:num list) bs' =
-          (((bir_exec_step_n birprog bs 0) = ([],0,bs')) ∧ (bs = bs'))) ∧ 
+          (((bir_exec_to_addr_label_n birprog bs 0) = (BER_Ended [] 0 0 bs')) ∧ (bs = bs'))) ∧ 
 (bir_mrel birprog bs beve bs' =
- ((bir_exec_step_n birprog bs (LENGTH beve)) = ([],(LENGTH beve),bs')))
+ ((bir_exec_to_addr_label_n birprog bs (LENGTH beve)) = (BER_Ended [] (LENGTH beve) (LENGTH beve) bs')))
 `;                                        
+*)
 
-(*
 Inductive bir_mrel:
 [~nil:]
- (bir_mrel p state [] state) /\
+ (bir_mrel p state [] state') /\
 [~moveForw:]
   (
   ((bir_mrel birprog bs bev bs'')∧(bir_rel birprog bs be bs'))
@@ -81,7 +84,7 @@ End
 val bir_mrel_single = new_axiom ("bir_mrel_single",
                                   ``∀birprog bs bev bs'. (bir_mrel birprog bs [bev] bs') = (bir_rel birprog bs bev bs')``);                                        
 
-
+(*
 val bir_mrel_def =
 Define `bir_mrel birprog bs beve bs' =
 (case beve of
@@ -114,16 +117,317 @@ val birprog_def = Define `
 val lifter_thm = REWRITE_RULE [GSYM arch_def,GSYM interval_def,GSYM arm8prog_def,GSYM birprog_def] XORexampleTheory.XORexample_thm;
 *)
 
+(* =================================================================================== *)
+
+(* NOTATION: FROM PROOF-PRODUCING SYMBOLIC EXECUTION -- adjusted/generalized from "bir_backlifterTheory.bir_is_lifted_prog_MULTI_STEP_EXEC_compute" *)
+(* =================================================================================== *)
+val bir_is_lifted_prog_MULTI_STEP_EXEC_compute_GEN_thm =
+  prove(
+  ``!mu bs bs' ms mla (p:'a bir_program_t) (r:('c, 'd, 'b) bir_lifting_machine_rec_t)
+      mms n' lo c_st c_addr_labels.
+    bir_is_lifted_prog r mu mms p ==>
+    bmr_rel r bs ms ==>
+    MEM (BL_Address mla) (bir_labels_of_program p) ==>
+    (bs.bst_pc = bir_block_pc (BL_Address mla)) ==>
+    EVERY (bmr_ms_mem_contains r ms) mms ==>
+    (bir_exec_to_addr_label_n p bs n' =
+         BER_Ended lo c_st c_addr_labels bs') ==>
+    ~bir_state_is_terminated bs ==>
+    ~bir_state_is_terminated bs' ==>
+    ?ms' li.
+    (FUNPOW_OPT r.bmr_step_fun c_addr_labels ms = SOME ms') /\
+    bmr_ms_mem_unchanged r ms ms' mu /\
+    EVERY (bmr_ms_mem_contains r ms') mms /\
+    (bs'.bst_pc = bir_block_pc (BL_Address li)) /\
+    MEM (BL_Address li) (bir_labels_of_program p) /\
+    bmr_rel r bs' ms'
+``,
+
+REPEAT STRIP_TAC >>
+ASSUME_TAC (ISPECL [``r:('c, 'd, 'b) bir_lifting_machine_rec_t``, ``mu:'c word_interval_t``,
+                    ``mms:(('c word)# ('d word) list) list``,
+                    ``p:'a bir_program_t``] bir_inst_liftingTheory.bir_is_lifted_prog_MULTI_STEP_EXEC) >>
+REV_FULL_SIMP_TAC std_ss [] >>
+bir_auxiliaryLib.QSPECL_X_ASSUM ``!n ms bs. _`` [`n'`, `ms`, `bs`] >>
+REV_FULL_SIMP_TAC (std_ss++holBACore_ss) [bir_programTheory.bir_state_is_terminated_def]
+);
+
+
+        
+val bir_is_lifted_prog_MULTI_STEP_EXEC_compute_32_8_thm =
+  INST_TYPE
+    [Type.gamma |-> ``:32``, Type.delta |-> ``:8``]
+    bir_is_lifted_prog_MULTI_STEP_EXEC_compute_GEN_thm;
+
+
+
+(*
+NOTATION: FROM PROOF-PRODUCING SYMBOLIC EXECUTION -- MULTISTEP WITH LABEL SET
+=======================================================
+*)
+
+(* n steps deterministic transition relation with using FUNPOW *)
+val step_n_def = Define `
+  (step_n stepf s n s' = (FUNPOW stepf n s = s'))
+`;
+
+val step_n_deterministic_thm = store_thm(
+   "step_n_deterministic_thm", ``
+!stepf.
+!s n s' s''.
+(step_n stepf s n s') ==>
+(step_n stepf s n s'') ==>
+(s' = s'')
+``,
+  SIMP_TAC std_ss [step_n_def]
+);
+val step_n_total_thm = store_thm(
+   "step_n_total_thm", ``
+!stepf.
+!s n.
+?s'.
+step_n stepf s n s'
+``,
+  SIMP_TAC std_ss [step_n_def]
+);
+
+val step_n_in_L_relaxed_def = Define `
+  step_n_in_L_relaxed pcf stepf s n L s' =
+    (step_n stepf s n s' /\
+     (n > 0) /\
+     (!n'. 0 < n' ==> n' < n ==>
+        ?s''. step_n stepf s n' s'' /\ pcf(s'') IN L))
+`;
+
+val step_n_in_L_def = Define `
+  step_n_in_L pcf stepf s n L s' =
+    ((pcf s) IN L /\
+     (step_n_in_L_relaxed pcf stepf s n L s'))
+`;
+
+val step_n_in_L_thm = save_thm("step_n_in_L_thm",
+  REWRITE_RULE [step_n_in_L_relaxed_def] step_n_in_L_def
+);
+
+val step_n_in_L_onlyL_thm = store_thm(
+   "step_n_in_L_onlyL_thm", ``
+!pcf stepf.
+!s n L s'.
+(step_n_in_L pcf stepf s n L s') ==>
+(
+  (* ((pcf s) IN L) /\ *)
+  (!n' s''. n' < n ==> step_n stepf s n' s'' ==> pcf(s'') IN L)
+)
+``,
+  SIMP_TAC std_ss [step_n_in_L_thm] >>
+  REPEAT STRIP_TAC >>
+  Cases_on `n'` >- (
+    FULL_SIMP_TAC std_ss [step_n_def, arithmeticTheory.FUNPOW]
+  ) >>
+  `0 < SUC n''` by (SIMP_TAC arith_ss []) >>
+  METIS_TAC [step_n_deterministic_thm]
+);
+
+val step_n_in_L_IMP_SUPER_thm = store_thm(
+   "step_n_in_L_IMP_SUPER_thm", ``
+!pcf stepf.
+!s n L L' s'.
+  (L SUBSET L') ==>
+  (step_n_in_L pcf stepf s n L  s') ==>
+  (step_n_in_L pcf stepf s n L' s')
+``,
+  REWRITE_TAC [step_n_in_L_thm, SUBSET_DEF] >>
+  METIS_TAC []
+);
+
+val step_n_in_L_SEQ_thm = store_thm(
+   "step_n_in_L_SEQ_thm", ``
+!pcf stepf.
+!s n_A L_A s' n_B L_B s''.
+  (step_n_in_L pcf stepf s  n_A L_A s') ==>
+  (step_n_in_L pcf stepf s' n_B L_B s'') ==>
+  (step_n_in_L pcf stepf s (n_A + n_B) (L_A UNION L_B) s'')
+``,
+  REWRITE_TAC [step_n_in_L_thm, step_n_def] >>
+  REPEAT STRIP_TAC >> (
+    ASM_SIMP_TAC (arith_ss++pred_setSimps.PRED_SET_ss) []
+  ) >> (
+    REWRITE_TAC [Once ADD_SYM] >>
+    ASM_SIMP_TAC (arith_ss++pred_setSimps.PRED_SET_ss) [step_n_def, FUNPOW_ADD]
+  ) >>
+
+  Cases_on `n' < n_A` >- (
+    METIS_TAC []
+  ) >>
+
+  (* n' = n_A + some difference *)
+  `?diff. n' = diff + n_A` by (
+    METIS_TAC [LESS_EQ_EXISTS, NOT_LESS, ADD_SYM]
+  ) >>
+
+  (* that difference < n_B *)
+  `diff < n_B` by (
+    ASM_SIMP_TAC (arith_ss) []
+  ) >>
+
+  (* with that, just solve with assumptions and FUNPOW_ADD *)
+  Cases_on `diff = 0` >> (
+    FULL_SIMP_TAC (arith_ss) [FUNPOW_ADD, FUNPOW_0]
+  )
+);
+
+val FUNPOW_ABS_thm = store_thm(
+   "FUNPOW_ABS_thm", ``
+!f g.
+  (!x. g (f x) = x) ==>
+  !stepf.
+  !s n s'.
+    FUNPOW (f o stepf o g) n (f s)
+    =
+    f (FUNPOW stepf n s)
+``,
+  REPEAT STRIP_TAC >>
+  FULL_SIMP_TAC std_ss [step_n_def] >>
+  Induct_on `n` >> (
+    FULL_SIMP_TAC std_ss [arithmeticTheory.FUNPOW_0, arithmeticTheory.FUNPOW_SUC]
+  )
+);
+
+val step_n_ABS_thm = store_thm(
+   "step_n_ABS_thm", ``
+!f g.
+  (!x y. (f x = f y) <=> (x = y)) ==>
+  (!x. g (f x) = x) ==>
+  !stepf.
+  !s n s'.
+    step_n (f o stepf o g) (f s) n (f s')
+    =
+    step_n stepf s n s'
+``,
+  FULL_SIMP_TAC std_ss [step_n_def, FUNPOW_ABS_thm]
+);
+
+val step_n_in_L_ABS_thm = store_thm(
+   "step_n_in_L_ABS_thm", ``
+!f g.
+  (!x y. (f x = f y) <=> (x = y)) ==>
+  (!x. g (f x) = x) ==>
+  (!x. ?y. (f y) = x) ==>
+  !pcf stepf.
+  !s n L s'.
+    step_n_in_L pcf (f o stepf o g) (f s) n L (f s')
+    =
+    step_n_in_L (pcf o f) stepf s n L s'
+``,
+  REPEAT STRIP_TAC >>
+  FULL_SIMP_TAC std_ss [step_n_in_L_def, step_n_in_L_relaxed_def] >>
+
+  EQ_TAC >> (
+    FULL_SIMP_TAC std_ss [step_n_ABS_thm] >>
+    REPEAT STRIP_TAC >>
+    PAT_X_ASSUM ``!x. A ==> B`` (ASSUME_TAC o Q.SPEC `n'`) >>
+    REV_FULL_SIMP_TAC std_ss [] >>
+    METIS_TAC [step_n_ABS_thm]
+  )
+);
+
+(*
+
+val bir_step_n_in_L_relaxed_def = Define `
+  bir_step_n_in_L_relaxed sr = step_n_in_L_relaxed symb_concst_pc sr.sr_step_conc
+`;
+        
+val conc_step_n_in_L_relaxed_def = Define `
+  conc_step_n_in_L_relaxed sr = step_n_in_L_relaxed symb_concst_pc sr.sr_step_conc
+`;
+
+val conc_step_n_in_L_def = Define `
+  conc_step_n_in_L sr = step_n_in_L symb_concst_pc sr.sr_step_conc
+`;
+
+val conc_step_n_in_L_IMP_relaxed_thm = store_thm(
+   "conc_step_n_in_L_IMP_relaxed_thm", ``
+!sr.
+!s n L s'.
+(conc_step_n_in_L sr s n L s') ==>
+(conc_step_n_in_L_relaxed sr s n L s')
+``,
+  METIS_TAC [conc_step_n_in_L_def, conc_step_n_in_L_relaxed_def, step_n_in_L_def]
+);
+
+
+        
+
+open bir_backlifterTheory;
+TODO: this is probably in precondition lifting
+"bir_backlifterTheory.exist_bir_of_arm8_thm"
+bir_backlifterTheory.bir_pre_arm8_to_bir_def
+bir_backlifterTheory.bir_post_bir_to_arm8_def
+((
+!ms.
+?bs.
+  (bir_envty_list_b birenvtyl st.bst_environ) /\
+  bmr_rel (m0_mod_bmr (F,T)) bs ms
+))
+bir_lifting_machinesTheory.m0_mod_bmr_def
+bir_exec_step_state_def
+bir_exec_step_def 
+step_n_def
+FUNPOW
+bir_exec_to_addr_label_n_def
+BER_Ended
+FUNPOW_OPT_def
+((
+``
+!bprog bs n L bs'.
+(step_n_in_L (\x. x.bst_pc) (bir_exec_step_state bprog) bs n L bs') ==>
+  ?n' lo.
+  (bir_exec_to_addr_label_n bprog bs n' = BER_Ended lo n n' bs')
+``
+REPEAT STRIP_TAC >>
+  FULL_SIMP_TAC std_ss [step_n_in_L_def] >>
+  FULL_SIMP_TAC std_ss [step_n_in_L_relaxed_def]
+  FULL_SIMP_TAC std_ss [step_n_def]
+FULL_SIMP_TAC std_ss [bir_exec_to_addr_label_n_def]
+  bir_exec_to_labels_n
+FULL_SIMP_TAC std_ss [bir_exec_step_state_def]
+FULL_SIMP_TAC std_ss [bir_exec_step_def
+  
+  FULL_SIMP_TAC std_ss [FUNPOW]
+))
+*)
+
+        
 val lifted_to_traces_thm = store_thm(
   "lifted_to_traces_thm",
-  ``∀interval arm8prog birprog.
-              (bir_is_lifted_prog arm8_bmr interval arm8prog birprog)
-     ==>
-     (∃ms bs ms' bs'.
-        (traces (bir_mrel birprog) bs bs') = (traces arm8_mrel ms ms')
+  ``!mu bs bs' ms ms' mla (p:'a bir_program_t)
+      mms n' lo c_st c_addr_labels.
+    bir_is_lifted_prog arm8_bmr mu mms p ==>
+    bmr_rel arm8_bmr bs ms ==>
+    MEM (BL_Address mla) (bir_labels_of_program p) ==>
+    (bs.bst_pc = bir_block_pc (BL_Address mla)) ==>
+    EVERY (bmr_ms_mem_contains arm8_bmr ms) mms ==>
+    (bir_exec_to_addr_label_n p bs n' =
+         BER_Ended lo c_st c_addr_labels bs') ==>
+    ~bir_state_is_terminated bs ==>
+    ~bir_state_is_terminated bs' ==>
+     (
+        (traces (bir_mrel p) bs bs') = (traces arm8_mrel ms ms')
      )
      ``,
      rpt strip_tac >>
+  IMP_RES_TAC bir_is_lifted_prog_MULTI_STEP_EXEC_compute_GEN_thm >>
+  FULL_SIMP_TAC (std_ss++listSimps.LIST_ss++pred_setSimps.PRED_SET_ss++boolSimps.LIFT_COND_ss++boolSimps.EQUIV_EXTRACT_ss++abstract_hoare_logicSimps.bir_wm_SS++holBACore_ss) [traces_def,MAP,IMAGE_DEF,EXTENSION] >>
+  Induct_on ‘x’ >- (
+    metis_tac[bir_mrel_nil,arm8_mrel_nil]
+    )(*NIL*) >>
+    GEN_TAC
+FULL_SIMP_TAC (std_ss++listSimps.LIST_ss++pred_setSimps.PRED_SET_ss++boolSimps.LIFT_COND_ss++boolSimps.EQUIV_EXTRACT_ss++abstract_hoare_logicSimps.bir_wm_SS++holBACore_ss) [TranRelSnocRev]
+
+                         
+
+Cases_on ‘c_addr_labels’
+        
      Cases_on ‘birprog’ >>
      Cases_on ‘interval’ >>
      FULL_SIMP_TAC (std_ss++listSimps.LIST_ss++pred_setSimps.PRED_SET_ss++boolSimps.LIFT_COND_ss++boolSimps.EQUIV_EXTRACT_ss++abstract_hoare_logicSimps.bir_wm_SS++holBACore_ss) [bmr_rel_def,bir_is_lifted_prog_def,bir_program_string_labels_guarded_def,bir_is_valid_labels_def,WI_wfe_def,bir_labels_of_program_def,bir_exec_to_addr_label_def,traces_def,MAP,EVERY_DEF,IMAGE_DEF,ALL_DISTINCT,EXTENSION,EVERY_CONJ,EVERY_FILTER,EXISTS_LIST_EQ_MAP,EVERY_MAP,arm8_bmr_def] >>
@@ -134,7 +438,8 @@ val lifted_to_traces_thm = store_thm(
      Induct_on ‘arm8prog’ >- (
       rewrite_tac[EVERY_DEF] >>
                  FULL_SIMP_TAC (std_ss++listSimps.LIST_ss++pred_setSimps.PRED_SET_ss++boolSimps.LIFT_COND_ss++boolSimps.EQUIV_EXTRACT_ss++abstract_hoare_logicSimps.bir_wm_SS++holBACore_ss) [bir_machine_lifted_imm_def,APPEND,arm8_PSTATE_lifted_imms_LIST_def,arm8_REGS_lifted_imms_LIST_def,arm8_EXTRA_lifted_imms_LIST_def] >>            
-
+      rw[]>>
+      RES_TAC
       )(*NIL*)
 
 
